src/IsoCan.v
@@ -4,6 +4,22 @@ Unset Strict Implicit.
 Unset Printing Implicit Defensive.
 From RDF Require Export Rdf Triple Term Util.
 
+(******************************************************************************)
+(* This file defines hashed data and its interaction with RDF graphs          *)
+(*                                                                            *)
+(* Hashed data is a polymorphic copy of pairs for which the first component   *)
+(* represents an initial blank node value; and its second component represents*)
+(* the current relabeling assigned to the initial value                       *)
+(*                                                                            *)
+(* For hashed data we define:                                                 *)
+(*  ** Predicate                                                              *)
+(*       eqb_b_hterm b ht          == b is the initial blank node value of ht *)
+(*                                                                            *)
+(*  ** Operations                                                             *)
+(*       lookup_hash_default h0 ht == the current hash of ht, or h0 if ht is  *)
+(*                                     not a blank node                       *)
+(*                                                                            *)
+(******************************************************************************)
 
 Section HashedData.
 
@@ -58,191 +74,192 @@ Section IsoCan.
 
   Implicit Type trm : term I B L.
 
-  Section IsoCanAlgorithm.
-    Variable disp2 : unit.
-    Variable h : orderType disp2.
-    Local Notation hash := (hash h).
+  Section inter.
 
-    Variable h0 : h.
+  Variable disp2 : unit.
+  Variable h : orderType disp2.
+  Local Notation hash := (hash h).
 
-    Definition init_bnode (b : B) : (hash B) :=
-      mkHinput b h0.
+  Variable h0 : h.
 
-    Lemma init_bnode_inj : injective init_bnode.
-    Proof. by move=> x y []. Qed.
+  Definition init_bnode (b : B) : (hash B) :=
+    mkHinput b h0.
 
-    Section Hterms.
+  Lemma init_bnode_inj : injective init_bnode.
+  Proof. by move=> x y []. Qed.
 
-      Definition hterm := term I (hash B) L.
+  Section Hterms.
 
-      Definition term_of_hterm (ht : hterm) : term I B L :=
-        match ht with
-        | Iri i => Iri i
-        | Bnode hb => Bnode (input hb)
-        | Lit l => Lit l
-        end.
+    Definition hterm := term I (hash B) L.
 
-      Definition eqb_trm_hi trm (ht : hterm) : bool := trm == (term_of_hterm ht).
+    Definition term_of_hterm (ht : hterm) : term I B L :=
+      match ht with
+      | Iri i => Iri i
+      | Bnode hb => Bnode (input hb)
+      | Lit l => Lit l
+      end.
 
-      Definition eqb_b_hterm (b : B) (ht : (term I (hash B) L)) : bool :=
-        if ht is Bnode hb then b == (input hb) else false.
+    Definition eqb_trm_hi trm (ht : hterm) : bool := trm == (term_of_hterm ht).
 
-      Lemma eqb_b_hterm_is_bnode b (ht : hterm) : eqb_b_hterm b ht -> is_bnode ht.
-      Proof. by case ht. Qed.
+    Definition eqb_b_hterm (b : B) (ht : (term I (hash B) L)) : bool :=
+      if ht is Bnode hb then b == (input hb) else false.
 
-      Lemma eqb_b_hterm_trans (b b': B) (ht : (term I (hash B) L)) :
-        eqb_b_hterm b ht -> eqb_b_hterm b' ht -> b = b'.
-      Proof. by case: ht=> // ? /eqP-> /eqP->. Qed.
+    Lemma eqb_b_hterm_is_bnode b (ht : hterm) : eqb_b_hterm b ht -> is_bnode ht.
+    Proof. by case ht. Qed.
 
-      Definition lookup_hash (hb : hterm) : option (hash B) :=
-        if hb is Bnode hin then some hin else None.
+    Lemma eqb_b_hterm_trans (b b': B) (ht : (term I (hash B) L)) :
+      eqb_b_hterm b ht -> eqb_b_hterm b' ht -> b = b'.
+    Proof. by case: ht=> // ? /eqP-> /eqP->. Qed.
 
-      Definition lookup_hash_default_ (hb : (term I (hash B) L) ) : h :=
-        if hb is Bnode hin then current_hash hin else h0.
+    Definition lookup_hash (hb : hterm) : option (hash B) :=
+      if hb is Bnode hin then some hin else None.
 
-      Definition eq_hash (b1 b2 : hterm) : bool :=
-        match (lookup_hash b1), (lookup_hash b2) with
-        | Some hin1, Some hin2 => current_hash hin1 == current_hash hin2
-        | _,_ => false
-        end.
+    Definition lookup_hash_default_ (hb : (term I (hash B) L) ) : h :=
+      if hb is Bnode hin then current_hash hin else h0.
 
-      Lemma eq_hash_refl b : is_bnode b -> eq_hash b b.
-      Proof. by case: b=> // ?; rewrite /eq_hash/= eqxx. Qed.
+    Definition eq_hash (b1 b2 : hterm) : bool :=
+      match (lookup_hash b1), (lookup_hash b2) with
+      | Some hin1, Some hin2 => current_hash hin1 == current_hash hin2
+      | _,_ => false
+      end.
 
-      Lemma eq_hash_refl_singl b g :
-        bnodes g = [:: b] ->
-        (if eq_hash b b then ([:: b], [::]) else ([::], [:: b])).1 = [:: b].
-      Proof. by move=> /b_in_bnode_is_bnode/eq_hash_refl ->. Qed.
+    Lemma eq_hash_refl b : is_bnode b -> eq_hash b b.
+    Proof. by case: b=> // ?; rewrite /eq_hash/= eqxx. Qed.
 
-      Definition cmp_bnode (b : B) (ht : hterm) : bool :=
-        match ht with
-        | Bnode hin => b == (input hin)
-        | _ => false
-        end.
+    Lemma eq_hash_refl_singl b g :
+      bnodes g = [:: b] ->
+      (if eq_hash b b then ([:: b], [::]) else ([::], [:: b])).1 = [:: b].
+    Proof. by move=> /b_in_bnode_is_bnode/eq_hash_refl ->. Qed.
 
-      Definition mu_ext (mu : B -> B) : (hash B) -> (hash B):=
-        fun b => (mkHinput (mu (input b)) (current_hash b)).
+    Definition cmp_bnode (b : B) (ht : hterm) : bool :=
+      match ht with
+      | Bnode hin => b == (input hin)
+      | _ => false
+      end.
 
-      Definition relabeling_hterm (mu : B -> B) ht : hterm :=
-        relabeling_term (mu_ext mu) ht.
+    Definition mu_ext (mu : B -> B) : (hash B) -> (hash B):=
+      fun b => (mkHinput (mu (input b)) (current_hash b)).
 
-      Lemma eqb_b_hterm_relabel f b ht (injF: injective f):
-        (eqb_b_hterm b ht) = (eqb_b_hterm (f b) (relabeling_hterm f ht)).
-      Proof. by case ht=> //= name; rewrite inj_eq. Qed.
+    Definition relabeling_hterm (mu : B -> B) ht : hterm :=
+      relabeling_term (mu_ext mu) ht.
 
-      Lemma has_map_eqbb s f b (injF: injective f):
-        has (eqb_b_hterm b) s = has (eqb_b_hterm (f b)) (map (relabeling_hterm f) s).
-      Proof. elim: s=> [//|hd tl IHtl] /=.
-             by rewrite IHtl (@eqb_b_hterm_relabel f b).
-      Qed.
+    Lemma eqb_b_hterm_relabel f b ht (injF: injective f):
+      (eqb_b_hterm b ht) = (eqb_b_hterm (f b) (relabeling_hterm f ht)).
+    Proof. by case ht=> //= name; rewrite inj_eq. Qed.
 
-    End Hterms.
-
-    Section Htriple.
-
-      Definition htriple := triple I (hash B) L.
-      Definition hts := seq (triple I (hash B) L).
-
-      Definition has_term_triple trm (trpl : htriple) : option hterm :=
-        match (filter (eqb_trm_hi trm) (terms_triple trpl)) with
-        | nil => None
-        | t :: ts => Some t
-        end.
-
-      Definition lookup_bnode_in_triple (b : B) (t : htriple) : option hterm :=
-        match (filter (cmp_bnode b) (terms_triple t)) with
-        | nil => None
-        | t :: ts => Some t
-        end.
-
-    End Htriple.
-
-    Section Hgraph.
-
-      Definition hgraph := rdf_graph I (hash_eqType h B) L.
-
-      Definition get t (g : hgraph) : option hterm :=
-        let otrs := (map (has_term_triple t) (graph g)) in
-        head None (filter isSome otrs).
-
-      Lemma init_hash_uniq {i l : eqType} (g : rdf_graph i B l) :
-        uniq (@relabeling_seq_triple i l _ _ init_bnode (graph g)).
-      Proof. by case g=> g' ug; rewrite map_inj_uniq //; apply: relabeling_triple_inj init_bnode_inj. Qed.
-
-      Definition init_hash_ts (ts : seq (triple I B L)) : hts :=
-        relabeling_seq_triple init_bnode ts.
-
-      Definition init_hash (g : rdf_graph _ _ _) : hgraph :=
-        @relabeling _ _ _ _ init_bnode g (init_hash_uniq g).
-
-      Lemma init_hash_ts_nil : init_hash_ts [::] = [::]. Proof. by []. Qed.
-
-      Lemma init_hash_nil : init_hash empty_rdf_graph = empty_rdf_graph. Proof. by apply rdf_inj. Qed.
-
-      Lemma init_hash_ts_h0 b g : Bnode b \in bnodes_ts (init_hash_ts g) -> current_hash b = h0.
-      Proof. by rewrite bnodes_ts_relabel_mem=> /map_inv [[]//? []->]. Qed.
-
-      Lemma init_hash_h0 b g : Bnode b \in bnodes (init_hash g) -> current_hash b = h0.
-      Proof. by apply init_hash_ts_h0. Qed.
-
-      Definition replace_bnode_ts (b b': hash B) (ts : hts) : hts :=
-        relabeling_seq_triple (fun a_hash => if a_hash == b then b' else a_hash) ts.
-
-      Definition replace_bnode (b b': hash B) (g : hgraph) us : hgraph :=
-        @mkRdfGraph _ _ _ (replace_bnode_ts b b' (graph g)) us.
-
-      Definition lookup_bnode_in_ts (ts : seq htriple) (b : B) : option hterm :=
-        let otrms := map (lookup_bnode_in_triple b) ts in
-        head None (filter isSome otrms).
-
-      Definition lookup_bnode_in_graph (g : hgraph) (b : B) : option hterm :=
-        lookup_bnode_in_ts (graph g) b.
-
-      Definition relabeling_hgraph (mu : B -> B) (g: hgraph) us : hgraph :=
-        @relabeling _ _ _ _ (mu_ext mu) g us.
-
-      Lemma eqb_b_hterm_relabeling b ht (mu : B -> B) :
-        eqb_b_hterm b ht ->
-        eqb_b_hterm (mu b) (relabeling_hterm mu ht).
-      Proof. by case: ht=> //? /eqP ->; rewrite /eqb_b_hterm/= eqxx. Qed.
-
-    End Hgraph.
-    Lemma nth_mapzip
-      (T1 T2 : Type) (S0 T0 : eqType)
-      (x0 : S0) (y0 : T0)
-      [s : seq S0] [t : seq T0] (i : nat) :
-      size s = size t ->
-        nth (@Bnode T1 (IsoCan.hash T0 S0) T2 (mkHinput x0 y0))
-            [seq Bnode (mkHinput an.1 an.2) | an <- zip s t ]
-            i =
-        Bnode (mkHinput (nth x0 s i) (nth y0 t i)).
-    Proof.
-      move=> eqsize.
-      case/orP : (leqVgt (size t) i)=> leq.
-      + suffices notin : (size [seq Bnode (mkHinput an.1 an.2) | an <- zip s t] <= i)%N.
-        by rewrite !nth_default // eqsize.
-        by move=> ? ? ; rewrite size_map size_zip eqsize minn_refl.
-        by rewrite (nth_map (x0,y0)) ?size_zip ?eqsize ?minn_refl // ; congr Bnode; apply/eqP; rewrite eq_i_ch /= nth_zip //= !eqxx.
+    Lemma has_map_eqbb s f b (injF: injective f):
+      has (eqb_b_hterm b) s = has (eqb_b_hterm (f b)) (map (relabeling_hterm f) s).
+    Proof. elim: s=> [//|hd tl IHtl] /=.
+           by rewrite IHtl (@eqb_b_hterm_relabel f b).
     Qed.
 
-    Lemma find_index_eqbb bs s (bn : B) :
-      size s = size bs ->
-      find (eqb_b_hterm bn) [seq Bnode (mkHinput an.1 an.2) | an <- zip bs s] = index bn bs.
-    Proof.
-      elim: bs s => [| a l IHl]; first by move=> ?; rewrite zip0s.
-      by case =>  [//| b l2] /= [eqsize_tl]; rewrite eq_sym IHl //.
-    Qed.
+  End Hterms.
 
-    Lemma hash_nth_mapzip
-      (U V : Type) (S0 T0 : eqType)
-      (x : S0) (y : T0)
-      [s : seq S0] [t : seq T0] (i : nat) :
-      size s = size t ->
-        nth (@Bnode U (IsoCan.hash T0 S0) V (mkHinput x y))
-            [seq Bnode (mkHinput an.1 an.2) | an <- zip s t ]
-            i =
-        Bnode (mkHinput (nth x s i) (nth y t i)).
+  Section Htriple.
+
+    Definition htriple := triple I (hash B) L.
+    Definition hts := seq (triple I (hash B) L).
+
+    Definition has_term_triple trm (trpl : htriple) : option hterm :=
+      match (filter (eqb_trm_hi trm) (terms_triple trpl)) with
+      | nil => None
+      | t :: ts => Some t
+      end.
+
+    Definition lookup_bnode_in_triple (b : B) (t : htriple) : option hterm :=
+      match (filter (cmp_bnode b) (terms_triple t)) with
+      | nil => None
+      | t :: ts => Some t
+      end.
+
+  End Htriple.
+
+  Section Hgraph.
+
+    Definition hgraph := rdf_graph I (hash_eqType h B) L.
+
+    Definition get t (g : hgraph) : option hterm :=
+      let otrs := (map (has_term_triple t) (graph g)) in
+      head None (filter isSome otrs).
+
+    Lemma init_hash_uniq {i l : eqType} (g : rdf_graph i B l) :
+      uniq (@relabeling_seq_triple i l _ _ init_bnode (graph g)).
+    Proof. by case g=> g' ug; rewrite map_inj_uniq //; apply: relabeling_triple_inj init_bnode_inj. Qed.
+
+    Definition init_hash_ts (ts : seq (triple I B L)) : hts :=
+      relabeling_seq_triple init_bnode ts.
+
+    Definition init_hash (g : rdf_graph _ _ _) : hgraph :=
+      @relabeling _ _ _ _ init_bnode g (init_hash_uniq g).
+
+    Lemma init_hash_ts_nil : init_hash_ts [::] = [::]. Proof. by []. Qed.
+
+    Lemma init_hash_nil : init_hash empty_rdf_graph = empty_rdf_graph. Proof. by apply rdf_inj. Qed.
+
+    Lemma init_hash_ts_h0 b g : Bnode b \in bnodes_ts (init_hash_ts g) -> current_hash b = h0.
+    Proof. by rewrite bnodes_ts_relabel_mem=> /map_inv [[]//? []->]. Qed.
+
+    Lemma init_hash_h0 b g : Bnode b \in bnodes (init_hash g) -> current_hash b = h0.
+    Proof. by apply init_hash_ts_h0. Qed.
+
+    Definition replace_bnode_ts (b b': hash B) (ts : hts) : hts :=
+      relabeling_seq_triple (fun a_hash => if a_hash == b then b' else a_hash) ts.
+
+    Definition replace_bnode (b b': hash B) (g : hgraph) us : hgraph :=
+      @mkRdfGraph _ _ _ (replace_bnode_ts b b' (graph g)) us.
+
+    Definition lookup_bnode_in_ts (ts : seq htriple) (b : B) : option hterm :=
+      let otrms := map (lookup_bnode_in_triple b) ts in
+      head None (filter isSome otrms).
+
+    Definition lookup_bnode_in_graph (g : hgraph) (b : B) : option hterm :=
+      lookup_bnode_in_ts (graph g) b.
+
+    Definition relabeling_hgraph (mu : B -> B) (g: hgraph) us : hgraph :=
+      @relabeling _ _ _ _ (mu_ext mu) g us.
+
+    Lemma eqb_b_hterm_relabeling b ht (mu : B -> B) :
+      eqb_b_hterm b ht ->
+      eqb_b_hterm (mu b) (relabeling_hterm mu ht).
+    Proof. by case: ht=> //? /eqP ->; rewrite /eqb_b_hterm/= eqxx. Qed.
+
+  End Hgraph.
+  Lemma nth_mapzip
+    (T1 T2 : Type) (S0 T0 : eqType)
+    (x0 : S0) (y0 : T0)
+    [s : seq S0] [t : seq T0] (i : nat) :
+    size s = size t ->
+    nth (@Bnode T1 (IsoCan.hash T0 S0) T2 (mkHinput x0 y0))
+      [seq Bnode (mkHinput an.1 an.2) | an <- zip s t ]
+      i =
+      Bnode (mkHinput (nth x0 s i) (nth y0 t i)).
+  Proof.
+    move=> eqsize.
+    case/orP : (leqVgt (size t) i)=> leq.
+    + suffices notin : (size [seq Bnode (mkHinput an.1 an.2) | an <- zip s t] <= i)%N.
+      by rewrite !nth_default // eqsize.
+      by move=> ? ? ; rewrite size_map size_zip eqsize minn_refl.
+      by rewrite (nth_map (x0,y0)) ?size_zip ?eqsize ?minn_refl // ; congr Bnode; apply/eqP; rewrite eq_i_ch /= nth_zip //= !eqxx.
+  Qed.
+
+  Lemma find_index_eqbb bs s (bn : B) :
+    size s = size bs ->
+    find (eqb_b_hterm bn) [seq Bnode (mkHinput an.1 an.2) | an <- zip bs s] = index bn bs.
+  Proof.
+    elim: bs s => [| a l IHl]; first by move=> ?; rewrite zip0s.
+    by case =>  [//| b l2] /= [eqsize_tl]; rewrite eq_sym IHl //.
+  Qed.
+
+  Lemma hash_nth_mapzip
+    (U V : Type) (S0 T0 : eqType)
+    (x : S0) (y : T0)
+    [s : seq S0] [t : seq T0] (i : nat) :
+    size s = size t ->
+    nth (@Bnode U (IsoCan.hash T0 S0) V (mkHinput x y))
+      [seq Bnode (mkHinput an.1 an.2) | an <- zip s t ]
+      i =
+      Bnode (mkHinput (nth x s i) (nth y t i)).
   Proof. by apply nth_mapzip. Qed.
+  End inter.
 
-  End IsoCanAlgorithm.
 End IsoCan.
